Use views consistently in the definition of rho (simpler proofs!)

pcuic/theories/PCUICRho.v
@@ -41,378 +41,530 @@ Section list_size.
   Qed.
 
 End list_size.
-  Lemma size_mkApps f l : size (mkApps f l) = size f + list_size size l.
-  Proof.
-    induction l in f |- *; simpl; try lia.
-    rewrite IHl. simpl. lia.
-  Qed.
+Lemma size_mkApps f l : size (mkApps f l) = size f + list_size size l.
+Proof.
+  induction l in f |- *; simpl; try lia.
+  rewrite IHl. simpl. lia.
+Qed.
 
-  Lemma list_size_app (l l' : list term) : list_size size (l ++ l') = list_size size l + list_size size l'.
-  Proof.
-    induction l; simpl; auto.
-    rewrite IHl. lia.
-  Qed.
+Lemma list_size_app (l l' : list term) : list_size size (l ++ l') = list_size size l + list_size size l'.
+Proof.
+  induction l; simpl; auto.
+  rewrite IHl. lia.
+Qed.
   
-  Section FoldFix.
-    Context (rho : context -> term -> term).
-    Context (Γ : context).
+Section FoldFix.
+  Context (rho : context -> term -> term).
+  Context (Γ : context).
 
-    Fixpoint fold_fix_context acc m :=
-      match m with
-      | [] => acc
-      | def :: fixd =>
-        fold_fix_context (vass def.(dname) (lift0 #|acc| (rho Γ def.(dtype))) :: acc) fixd
-      end.
-  End FoldFix.
+  Fixpoint fold_fix_context acc m :=
+    match m with
+  | [] => acc
+    | def :: fixd =>
+      fold_fix_context (vass def.(dname) (lift0 #|acc| (rho Γ def.(dtype))) :: acc) fixd
+    end.
+End FoldFix.
 
-  Fixpoint isFixLambda_app (t : term) : bool :=
-    match t with
-    | tApp (tFix _ _) _ => true
-    | tApp (tLambda _ _ _) _ => true 
-    | tApp f _ => isFixLambda_app f
-    | _ => false
+Fixpoint isFixLambda_app (t : term) : bool :=
+match t with
+| tApp (tFix _ _) _ => true
+| tApp (tLambda _ _ _) _ => true 
+| tApp f _ => isFixLambda_app f
+| _ => false
+end.
+
+Inductive fix_lambda_app_view : term -> term -> Type :=
+| fix_lambda_app_fix mfix i l a : fix_lambda_app_view (mkApps (tFix mfix i) l) a
+| fix_lambda_app_lambda na ty b l a : fix_lambda_app_view (mkApps (tLambda na ty b) l) a
+| fix_lambda_app_other t a : ~~ isFixLambda_app (tApp t a) -> fix_lambda_app_view t a.
+Derive Signature for fix_lambda_app_view.
+
+Lemma view_lambda_fix_app (t u : term) : fix_lambda_app_view t u.
+Proof.
+induction t; try solve [apply fix_lambda_app_other; simpl; auto].
+apply (fix_lambda_app_lambda na t1 t2 [] u).
+destruct IHt1.
+pose proof (fix_lambda_app_fix mfix i (l ++ [t2]) a).
+now rewrite -mkApps_nested in X.
+pose proof (fix_lambda_app_lambda na ty b (l ++ [t2]) a).
+now rewrite -mkApps_nested in X.
+destruct t; try solve [apply fix_lambda_app_other; simpl; auto].
+apply (fix_lambda_app_fix mfix idx [] u).
+Qed.
+
+Equations construct_cofix_discr (t : term) : bool :=
+construct_cofix_discr (tConstruct _ _ _) => true;
+construct_cofix_discr (tCoFix _ _) => true;
+construct_cofix_discr _ => false.
+Transparent construct_cofix_discr.
+
+Equations discr_construct_cofix (t : term) : Prop :=
+  { | tConstruct _ _ _ => False;
+    | tCoFix _ _ => False;
+    | _ => True }.
+Transparent discr_construct_cofix.
+
+Inductive construct_cofix_view : term -> Type :=
+| construct_cofix_construct c u i : construct_cofix_view (tConstruct c u i)
+| construct_cofix_cofix mfix idx : construct_cofix_view (tCoFix mfix idx)
+| construct_cofix_other t : discr_construct_cofix t -> construct_cofix_view t.
+
+Equations view_construct_cofix (t : term) : construct_cofix_view t :=
+{ | tConstruct ind u i => construct_cofix_construct ind u i;
+  | tCoFix mfix idx => construct_cofix_cofix mfix idx;
+  | t => construct_cofix_other t I }.
+
+Section Rho.
+  Context (Σ : global_env).
+
+  #[program] Definition map_fix_rho {t} (rho : context -> forall x, size x < size t -> term) Γ mfixctx (mfix : mfixpoint term)
+    (H : mfixpoint_size size mfix < size t) :=
+    (map_In mfix (fun d (H : In d mfix) => {| dname := dname d; 
+        dtype := rho Γ (dtype d) _;
+        dbody := rho (Γ ,,, mfixctx) (dbody d) _; rarg := (rarg d) |})).
+  Next Obligation.
+    eapply (In_list_size (def_size size)) in H.
+    eapply le_lt_trans with (def_size size d).
+    unfold def_size. lia.
+    unfold mfixpoint_size in H0.
+    lia.
+  Qed.
+  Next Obligation.
+    eapply (In_list_size (def_size size)) in H.
+    eapply le_lt_trans with (def_size size d).
+    unfold def_size. lia.
+    unfold mfixpoint_size in H0.
+    lia.
+  Qed.
+
+  Equations? fold_fix_context_wf mfix 
+      (rho : context -> forall x, size x < (mfixpoint_size size mfix) -> term) 
+      (Γ acc : context) : context :=
+  fold_fix_context_wf [] rho Γ acc => acc ;
+  fold_fix_context_wf (d :: mfix) rho Γ acc => 
+    fold_fix_context_wf mfix (fun Γ x Hx => rho Γ x _) Γ (vass (dname d) (lift0 #|acc| (rho Γ (dtype d) _)) :: acc).
+  Proof.
+    lia. unfold def_size. lia.        
+  Qed.
+  Transparent fold_fix_context_wf.
+
+  #[program] Definition map_terms {t} (rho : context -> forall x, size x < size t -> term) Γ (l : list term)
+    (H : list_size size l < size t) :=
+    (map_In l (fun t (H : In t l) => rho Γ t _)).
+  Next Obligation.
+    eapply (In_list_size size) in H. lia.
+  Qed.
+
+  #[program] Definition map_brs {t} (rho : context -> forall x, size x < size t -> term) Γ (l : list (nat * term))
+    (H : list_size (fun x : nat * term => size x.2) l < size t) :=
+  (map_In l (fun x (H : In x l) => (x.1, rho Γ x.2 _))).
+  Next Obligation.
+    eapply (In_list_size (fun x => size x.2)) in H. simpl in *. lia.
+  Qed.
+
+  Definition inspect {A} (x : A) : { y : A | y = x } := exist x eq_refl.
+
+  Definition unfold_fix mfix idx :=
+    match nth_error mfix idx with
+    | Some d => Some (rarg d, subst0 (fix_subst mfix) (dbody d))
+    | None => None
     end.
 
-  Inductive fix_lambda_app_view : term -> term -> Type :=
-  | fix_lambda_app_fix mfix i l a : fix_lambda_app_view (mkApps (tFix mfix i) l) a
-  | fix_lambda_app_lambda na ty b l a : fix_lambda_app_view (mkApps (tLambda na ty b) l) a
-  | fix_lambda_app_other t a : ~~ isFixLambda_app (tApp t a) -> fix_lambda_app_view t a.
+  Equations? rho (Γ : context) (t : term) : term by wf (size t) := 
+  rho Γ (tApp t u) with view_lambda_fix_app t u := 
+    { | fix_lambda_app_lambda na T b [] u' := 
+        (rho (vass na (rho Γ T) :: Γ) b) {0 := rho Γ u'};
+      | fix_lambda_app_lambda na T b (a :: l) u' :=
+        mkApps ((rho (vass na (rho Γ T) :: Γ) b) {0 := rho Γ a})
+          (map_terms rho Γ (l ++ [u']) _);
+      | fix_lambda_app_fix mfix idx l a :=
+        let mfixctx := fold_fix_context_wf mfix (fun Γ x Hx => rho Γ x) Γ [] in 
+        let mfix' := map_fix_rho (t:=tFix mfix idx) (fun Γ x Hx => rho Γ x) Γ mfixctx mfix _ in
+        let args := map_terms rho Γ (l ++ [a]) _ in
+        match unfold_fix mfix' idx with 
+        | Some (rarg, fn) =>
+          if is_constructor rarg (l ++ [a]) then
+            mkApps fn args
+          else mkApps (tFix mfix' idx) args
+        | None => mkApps (tFix mfix' idx) args
+        end ;
+      | fix_lambda_app_other t' u' nisfixlam := tApp (rho Γ t') (rho Γ u') } ; 
+  rho Γ (tLetIn na d t b) => (subst10 (rho Γ d) (rho (vdef na (rho Γ d) (rho Γ t) :: Γ) b)); 
+  rho Γ (tRel i) with option_map decl_body (nth_error Γ i) := { 
+    | Some (Some body) => (lift0 (S i) body); 
+    | Some None => tRel i; 
+    | None => tRel i }; 
 
-  Lemma view_lambda_fix_app (t u : term) : fix_lambda_app_view t u.
+  rho Γ (tCase (ind, pars) p x brs) with inspect (decompose_app x) :=
+  { | exist (f, args) eqx with view_construct_cofix f := 
+  { | construct_cofix_construct ind' c u with eq_inductive ind ind' := 
+    { | true => 
+        let p' := rho Γ p in 
+        let args' := map_terms rho Γ args _ in 
+        let brs' := map_brs rho Γ brs _ in 
+        iota_red pars c args' brs'; 
+      | false => 
+        let p' := rho Γ p in 
+        let x' := rho Γ x in 
+        let brs' := map_brs rho Γ brs _ in 
+        tCase (ind, pars) p' x' brs' }; 
+    | construct_cofix_cofix mfix idx :=
+      let p' := rho Γ p in 
+      let args' := map_terms rho Γ args _ in 
+      let brs' := map_brs rho Γ brs _ in 
+      let mfixctx := fold_fix_context_wf mfix (fun Γ x Hx => rho Γ x) Γ [] in 
+      let mfix' := map_fix_rho (t:=tCase (ind, pars) p x brs) rho Γ mfixctx mfix _ in
+        match nth_error mfix' idx with
+        | Some d =>
+          tCase (ind, pars) p' (mkApps (subst0 (cofix_subst mfix') (dbody d)) args') brs'
+        | None => tCase (ind, pars) p' (rho Γ x) brs'
+        end; 
+    | construct_cofix_other t nconscof => 
+      let p' := rho Γ p in 
+      let x' := rho Γ x in 
+      let brs' := map_brs rho Γ brs _ in 
+        tCase (ind, pars) p' x' brs' } };
+
+  rho Γ (tProj (i, pars, narg) x) with inspect (decompose_app x) := {
+    | exist (f, args) eqx with view_construct_cofix f :=
+    | construct_cofix_construct ind c u with inspect (nth_error (map_terms rho Γ args _) (pars + narg)) := { 
+      | exist (Some arg1) eq => 
+        if eq_inductive i ind then arg1
+        else tProj (i, pars, narg) (rho Γ x);
+      | exist None neq => tProj (i, pars, narg) (rho Γ x) }; 
+    | construct_cofix_cofix mfix idx := 
+      let args' := map_terms rho Γ args _ in
+      let mfixctx := fold_fix_context_wf mfix (fun Γ x Hx => rho Γ x) Γ [] in 
+      let mfix' := map_fix_rho (t:=tProj (i, pars, narg) x) rho Γ mfixctx mfix _ in
+      match nth_error mfix' idx with
+      | Some d => tProj (i, pars, narg) (mkApps (subst0 (cofix_subst mfix') (dbody d)) args')
+      | None =>  tProj (i, pars, narg) (rho Γ x)
+      end;
+    | construct_cofix_other t nconscof => tProj (i, pars, narg) (rho Γ x) } ;
+  rho Γ (tConst c u) with lookup_env Σ c := { 
+    | Some (ConstantDecl decl) with decl.(cst_body) := { 
+      | Some body => subst_instance_constr u body; 
+      | None => tConst c u }; 
+    | _ => tConst c u }; 
+  rho Γ (tLambda na t u) => tLambda na (rho Γ t) (rho (vass na (rho Γ t) :: Γ) u); 
+  rho Γ (tProd na t u) => tProd na (rho Γ t) (rho (vass na (rho Γ t) :: Γ) u); 
+  rho Γ (tVar i) => tVar i; 
+  rho Γ (tEvar n l) => tEvar n (map_terms rho Γ l _); 
+  rho Γ (tSort s) => tSort s; 
+  rho Γ (tFix mfix idx) => 
+    let mfixctx := fold_fix_context_wf mfix (fun Γ x Hx => rho Γ x) Γ [] in 
+    tFix (map_fix_rho (t:=tFix mfix idx) (fun Γ x Hx => rho Γ x) Γ mfixctx mfix _) idx; 
+  rho Γ (tCoFix mfix idx) => 
+    let mfixctx := fold_fix_context_wf mfix (fun Γ x Hx => rho Γ x) Γ [] in 
+    tCoFix (map_fix_rho (t:=tCoFix mfix idx) rho Γ mfixctx mfix _) idx; 
+  rho Γ x => x.
   Proof.
-    induction t; try solve [apply fix_lambda_app_other; simpl; auto].
-    apply (fix_lambda_app_lambda na t1 t2 [] u).
-    destruct IHt1.
-    pose proof (fix_lambda_app_fix mfix i (l ++ [t2]) a).
-    now rewrite -mkApps_nested in X.
-    pose proof (fix_lambda_app_lambda na ty b (l ++ [t2]) a).
-    now rewrite -mkApps_nested in X.
-    destruct t; try solve [apply fix_lambda_app_other; simpl; auto].
-    apply (fix_lambda_app_fix mfix idx [] u).
+    all:try abstract lia.
+    - abstract (rewrite size_mkApps ?list_size_app /=; lia).
+    - simpl in Hx. abstract (rewrite size_mkApps /=; lia).
+    - clear; abstract (rewrite list_size_app size_mkApps /=; lia).
+    - clear; abstract (rewrite size_mkApps /=; lia).
+    - clear; abstract (rewrite size_mkApps /=; lia).
+    - clear; abstract (rewrite size_mkApps /=; lia).
+    - clear; abstract (rewrite list_size_app size_mkApps /=; lia).
+    - clear -eqx; eapply symmetry, decompose_app_inv in eqx. subst x. 
+      abstract (rewrite size_mkApps /=; lia).
+    - clear; abstract (lia).
+    - clear -eqx; eapply symmetry, decompose_app_inv in eqx. subst x. 
+      abstract (rewrite size_mkApps /=; lia).
+    - clear. abstract lia.      
+    - clear -eqx Hx. eapply symmetry, decompose_app_inv in eqx; subst x0.
+      abstract (rewrite size_mkApps /=; lia).
+    - clear -eqx. eapply symmetry, decompose_app_inv in eqx; subst x.
+      abstract (rewrite size_mkApps /=; lia).
+    - clear -eqx. eapply symmetry, decompose_app_inv in eqx; subst x.
+      abstract (rewrite size_mkApps /=; lia).
+    - clear -eqx. eapply symmetry, decompose_app_inv in eqx; subst x.
+      abstract (rewrite size_mkApps /=; lia).
+    - clear -eqx. eapply symmetry, decompose_app_inv in eqx; subst x.
+      abstract (rewrite size_mkApps /=; lia).
+    - clear -eqx Hx. eapply symmetry, decompose_app_inv in eqx; subst x0.
+      abstract (rewrite size_mkApps /=; lia).
+    - clear -eqx. eapply symmetry, decompose_app_inv in eqx; subst x.
+      abstract (rewrite size_mkApps /=; lia). 
+  Defined.
+
+  Lemma map_terms_map t Γ l H : @map_terms t (fun Γ x Hx => rho Γ x) Γ l H = map (rho Γ) l. 
+  Proof. 
+    unfold map_terms. now rewrite map_In_spec.
+  Qed. 
+  Hint Rewrite map_terms_map : rho.
+
+  Lemma map_brs_map t Γ l H : @map_brs t (fun Γ x Hx => rho Γ x) Γ l H = map (fun x => (x.1, rho Γ x.2)) l. 
+  Proof. 
+    unfold map_brs. now rewrite map_In_spec.
+  Qed. 
+  Hint Rewrite map_brs_map : rho.
+
+  Definition map_fix (rho : context -> term -> term) Γ mfixctx (mfix : mfixpoint term) :=
+    (map (map_def (rho Γ) (rho (Γ ,,, mfixctx))) mfix).
+
+  Lemma map_fix_rho_map t Γ mfix ctx H : 
+    @map_fix_rho t (fun Γ x Hx => rho Γ x) Γ ctx mfix H = 
+    map_fix rho Γ ctx mfix.
+  Proof. 
+    unfold map_fix_rho. now rewrite map_In_spec.
   Qed.
 
-  Section Rho.
-    Context (Σ : global_env).
+  Lemma fold_fix_context_wf_fold mfix Γ ctx :
+    fold_fix_context_wf mfix (fun Γ x _ => rho Γ x) Γ ctx = 
+    fold_fix_context rho Γ ctx mfix.
+  Proof.
+    induction mfix in ctx |- *; simpl; auto. 
+  Qed.
 
-    #[program] Definition map_fix_rho {t} (rho : context -> forall x, size x < size t -> term) Γ mfixctx (mfix : mfixpoint term)
-      (H : mfixpoint_size size mfix < size t) :=
-      (map_In mfix (fun d (H : In d mfix) => {| dname := dname d; 
-          dtype := rho Γ (dtype d) _;
-          dbody := rho (Γ ,,, mfixctx) (dbody d) _; rarg := (rarg d) |})).
-    Next Obligation.
-      eapply (In_list_size (def_size size)) in H.
-      eapply le_lt_trans with (def_size size d).
-      unfold def_size. lia.
-      unfold mfixpoint_size in H0.
-      lia.
-    Qed.
-    Next Obligation.
-      eapply (In_list_size (def_size size)) in H.
-      eapply le_lt_trans with (def_size size d).
-      unfold def_size. lia.
-      unfold mfixpoint_size in H0.
-      lia.
-    Qed.
+  Hint Rewrite map_fix_rho_map fold_fix_context_wf_fold : rho.
 
-    Equations? fold_fix_context_wf mfix 
-        (rho : context -> forall x, size x < (mfixpoint_size size mfix) -> term) 
-        (Γ acc : context) : context :=
-    fold_fix_context_wf [] rho Γ acc => acc ;
-    fold_fix_context_wf (d :: mfix) rho Γ acc => 
-      fold_fix_context_wf mfix (fun Γ x Hx => rho Γ x _) Γ (vass (dname d) (lift0 #|acc| (rho Γ (dtype d) _)) :: acc).
-    Proof.
-      lia. unfold def_size. lia.        
-    Qed.
-    Transparent fold_fix_context_wf.
+  Lemma mkApps_tApp f a l : mkApps (tApp f a) l = mkApps f (a :: l).
+  Proof. reflexivity. Qed.
 
-    #[program] Definition map_terms {t} (rho : context -> forall x, size x < size t -> term) Γ (l : list term)
-      (H : list_size size l < size t) :=
-      (map_In l (fun t (H : In t l) => rho Γ t _)).
-    Next Obligation.
-      eapply (In_list_size size) in H. lia.
-    Qed.
+  Lemma tApp_mkApps f a : tApp f a = mkApps f [a].
+  Proof. reflexivity. Qed.
+
+  Lemma isFixLambda_app_mkApps t l : isFixLambda_app t -> isFixLambda_app (mkApps t l).
+  Proof. 
+    induction l using rev_ind; simpl; auto.
+    rewrite -mkApps_nested. 
+    intros isf. specialize (IHl isf).
+    simpl. rewrite IHl. destruct (mkApps t l); auto.
+  Qed.
+  Definition isFixLambda (t : term) : bool :=
+  match t with
+  | tFix _ _ => true
+  | tLambda _ _ _ => true
+  | _ => false
+  end.
+
+  Inductive fix_lambda_view : term -> Type :=
+  | fix_lambda_lambda na b t : fix_lambda_view (tLambda na b t)
+  | fix_lambda_fix mfix i : fix_lambda_view (tFix mfix i)
+  | fix_lambda_other t : ~~ isFixLambda t -> fix_lambda_view t.
+
+  Lemma view_fix_lambda (t : term) : fix_lambda_view t.
+  Proof.
+    destruct t; repeat constructor.
+  Qed.
   
-    #[program] Definition map_brs {t} (rho : context -> forall x, size x < size t -> term) Γ (l : list (nat * term))
-      (H : list_size (fun x : nat * term => size x.2) l < size t) :=
-    (map_In l (fun x (H : In x l) => (x.1, rho Γ x.2 _))).
-    Next Obligation.
-      eapply (In_list_size (fun x => size x.2)) in H. simpl in *. lia.
-    Qed.
+  Lemma isFixLambda_app_mkApps' t l x : isFixLambda t -> isFixLambda_app (tApp (mkApps t l) x).
+  Proof. 
+    induction l using rev_ind; simpl; auto.
+    destruct t; auto.
+    intros isl. specialize (IHl isl).
+    simpl in IHl.
+    now rewrite -mkApps_nested /=. 
+  Qed.
 
-    Definition inspect {A} (x : A) : { y : A | y = x } := exist x eq_refl.
+  Ltac solve_discr := (try (progress (prepare_discr; finish_discr; cbn [mkApps] in * )));
+      try discriminate.
 
-    Definition unfold_fix mfix idx :=
+  Ltac discr_mkApps H := 
+    let Hf := fresh in let Hargs := fresh in
+    rewrite ?tApp_mkApps ?mkApps_nested in H;
+      (eapply mkApps_nApp_inj in H as [Hf Hargs] ||
+        eapply (mkApps_nApp_inj _ _ []) in H as [Hf Hargs] ||
+        eapply (mkApps_nApp_inj _ _ _ []) in H as [Hf Hargs]);
+        [noconf Hf|reflexivity].
+
+  Set Equations With UIP. (* This allows to use decidable equality on terms. *)
+
+  (* Most of this is discrimination, we should have a more robust tactic to  
+    solve this. *)
+  Lemma rho_app_lambda Γ na ty b a l :
+    rho Γ (mkApps (tApp (tLambda na ty b) a) l) =  
+    mkApps ((rho (vass na (rho Γ ty) :: Γ) b) {0 := rho Γ a}) (map (rho Γ) l).
+  Proof.
+    induction l using rev_ind; autorewrite with rho.
+    - set (view := view_lambda_fix_app _ _). clearbody view.
+      depelim view. injection H. intros. discr_mkApps H1.
+      injection H. intros. discr_mkApps H1. subst.
+      now simpl in H; noconf H.
+      simpl in i; discriminate.
+    - simpl. rewrite -mkApps_nested. autorewrite with rho.
+      set (view := view_lambda_fix_app _ _). clearbody view.
+      depelim view. injection H. intros. discr_mkApps H1.
+      injection H. intros. discr_mkApps H1. subst. clear H.
+      remember (mkApps (tApp (tLambda na ty b) a) l).
+      depelim view0. discr_mkApps Heqt.
+      discr_mkApps Heqt. subst. simpl. now autorewrite with rho.
+      subst t. elimtype False. rewrite !tApp_mkApps mkApps_nested in i.
+      rewrite isFixLambda_app_mkApps in i => //.
+      elimtype False; rewrite !tApp_mkApps mkApps_nested in i.
+      rewrite isFixLambda_app_mkApps in i => //.
+  Qed.
+  
+  Lemma map_cofix_subst (f : context -> term -> term)
+        (f' : context -> context -> term -> term) mfix Γ Γ' :
+    (forall n, tCoFix (map (map_def (f Γ) (f' Γ Γ')) mfix) n = f Γ (tCoFix mfix n)) ->
+    cofix_subst (map (map_def (f Γ) (f' Γ Γ')) mfix) =
+    map (f Γ) (cofix_subst mfix).
+  Proof.
+    unfold cofix_subst. intros.
+    rewrite map_length. generalize (#|mfix|). induction n. simpl. reflexivity.
+    simpl. rewrite - IHn. f_equal. apply H.
+  Qed.
+
+  Lemma map_fix_subst f g mfix :
+    (forall n, tFix (map (map_def f g) mfix) n = f (tFix mfix n)) ->
+    fix_subst (map (map_def f g) mfix) =
+    map f (fix_subst mfix).
+  Proof.
+    unfold fix_subst. intros.
+    rewrite map_length. generalize (#|mfix|) at 1 2. induction n. simpl. reflexivity.
+    simpl. rewrite - IHn. f_equal. apply H.
+  Qed.
+
+  Lemma rho_app_fix Γ mfix idx args :
+    let rhoargs := map (rho Γ) args in
+    rho Γ (mkApps (tFix mfix idx) args) = 
       match nth_error mfix idx with
-      | Some d => Some (rarg d, subst0 (fix_subst mfix) (dbody d))
-      | None => None
+      | Some d => 
+        if is_constructor (rarg d) args then 
+          let fn := (subst0 (map (rho Γ) (fix_subst mfix))) (rho (Γ ,,, fold_fix_context rho Γ [] mfix) (dbody d)) in
+          mkApps fn rhoargs
+        else mkApps (rho Γ (tFix mfix idx)) rhoargs
+      | None => mkApps (rho Γ (tFix mfix idx)) rhoargs
       end.
-
-    Equations? rho (Γ : context) (t : term) : term by wf (size t) := 
-       { rho Γ (tApp t u) with view_lambda_fix_app t u := 
-           { | fix_lambda_app_lambda na T b [] u' := 
-                (rho (vass na (rho Γ T) :: Γ) b) {0 := rho Γ u'};
-             | fix_lambda_app_lambda na T b (a :: l) u' :=
-                mkApps ((rho (vass na (rho Γ T) :: Γ) b) {0 := rho Γ a})
-                  (map_terms rho Γ (l ++ [u']) _);
-             | fix_lambda_app_fix mfix idx l a :=
-               let mfixctx := fold_fix_context_wf mfix (fun Γ x Hx => rho Γ x) Γ [] in 
-               let mfix' := map_fix_rho (t:=tFix mfix idx) (fun Γ x Hx => rho Γ x) Γ mfixctx mfix _ in
-               let args := map_terms rho Γ (l ++ [a]) _ in
-               match unfold_fix mfix' idx with 
-                | Some (rarg, fn) =>
-                  if is_constructor rarg (l ++ [a]) then
-                    mkApps fn args
-                  else mkApps (tFix mfix' idx) args
-                | None => mkApps (tFix mfix' idx) args
-                end ;
-             | fix_lambda_app_other t' u' nisfixlam := tApp (rho Γ t') (rho Γ u') } ; 
-       rho Γ (tLetIn na d t b) => (subst10 (rho Γ d) (rho (vdef na (rho Γ d) (rho Γ t) :: Γ) b)); 
-       rho Γ (tRel i) with option_map decl_body (nth_error Γ i) := { 
-         | Some (Some body) => (lift0 (S i) body); 
-         | Some None => tRel i; 
-         | None => tRel i }; 
-       rho Γ (tCase (ind, pars) p x brs) with decompose_app x, decompose_app (rho Γ x) := 
-         { | (tConstruct ind' c u, args) | (tConstruct ind'' c' u', args') 
-          with eq_inductive ind ind' := 
-          { | true => 
-              let p' := rho Γ p in 
-              let x' := rho Γ x in 
-              let brs' := map_brs rho Γ brs _ in 
-              iota_red pars c args' brs'; 
-            | false => 
-              let p' := rho Γ p in 
-              let x' := rho Γ x in 
-              let brs' := map_brs rho Γ brs _ in 
-              tCase (ind, pars) p' x' brs' }; 
-       | (tCoFix mfix idx, args) | (tCoFix mfix' idx', args') with unfold_cofix mfix' idx := { 
-         | Some (narg, fn) => 
-           let p' := rho Γ p in 
-           let x' := rho Γ x in 
-           let brs' := map_brs rho Γ brs _ in 
-           tCase (ind, pars) p' (mkApps fn args') brs'; 
-         | None => 
-           let p' := rho Γ p in 
-           let x' := rho Γ x in 
-           let brs' := map_brs rho Γ brs _ in 
-           tCase (ind, pars) p' (mkApps (tCoFix mfix' idx) args') brs' }; 
-       | _ | _ => 
-             let p' := rho Γ p in 
-             let x' := rho Γ x in 
-             let brs' := map_brs rho Γ brs _ in 
-             tCase (ind, pars) p' x' brs' }; 
-     rho Γ (tProj (i, pars, narg) x) with decompose_app x, decompose_app (rho Γ x) := { 
-       | (tConstruct ind c u, args) | (tConstruct ind' c' u', args') with 
-         nth_error args' (pars + narg) := { 
-         | Some arg1 => 
-           if eq_inductive i ind' then arg1 
-           else tProj (i, pars, narg) (rho Γ x); 
-      | None => tProj (i, pars, narg) (rho Γ x) }; 
-       | (tCoFix mfix idx, args) | (tCoFix mfix' idx', args') with unfold_cofix mfix' idx := { 
-         | Some (narg, fn) => tProj (i, pars, narg) (mkApps fn args'); 
-         | None => tProj (i, pars, narg) (mkApps (tCoFix mfix' idx') args') }; 
-       | _ | _ => tProj (i, pars, narg) (rho Γ x) }; 
-    rho Γ (tConst c u) with lookup_env Σ c := { 
-       | Some (ConstantDecl decl) with decl.(cst_body) := { 
-         | Some body => subst_instance_constr u body; 
-         | None => tConst c u }; 
-       | _ => tConst c u }; 
-     rho Γ (tLambda na t u) => tLambda na (rho Γ t) (rho (vass na (rho Γ t) :: Γ) u); 
-     rho Γ (tProd na t u) => tProd na (rho Γ t) (rho (vass na (rho Γ t) :: Γ) u); 
-     rho Γ (tVar i) => tVar i; 
-     rho Γ (tEvar n l) => tEvar n (map_terms rho Γ l _); 
-     rho Γ (tSort s) => tSort s; 
-     rho Γ (tFix mfix idx) => 
-       let mfixctx := fold_fix_context_wf mfix (fun Γ x Hx => rho Γ x) Γ [] in 
-       tFix (map_fix_rho (t:=tFix mfix idx) (fun Γ x Hx => rho Γ x) Γ mfixctx mfix _) idx; 
-     rho Γ (tCoFix mfix idx) => 
-       let mfixctx := fold_fix_context_wf mfix (fun Γ x Hx => rho Γ x) Γ [] in 
-       tCoFix (map_fix_rho (t:=tCoFix mfix idx) rho Γ mfixctx mfix _) idx; 
-       rho Γ x => x }.
-    Proof.
-      all:try abstract lia.
-      - abstract (rewrite size_mkApps ?list_size_app /=; lia).
-      - simpl in Hx. abstract (rewrite size_mkApps /=; lia).
-      - abstract (rewrite list_size_app size_mkApps /=; lia).
-      - abstract (rewrite size_mkApps /=; lia).
-      - abstract (rewrite size_mkApps /=; lia).
-      - abstract (rewrite size_mkApps /=; lia).
-      - abstract (rewrite list_size_app size_mkApps /=; lia).
-    Defined.
-
-    Lemma map_terms_map t Γ l H : @map_terms t (fun Γ x Hx => rho Γ x) Γ l H = map (rho Γ) l. 
-    Proof. 
-      unfold map_terms. now rewrite map_In_spec.
-    Qed. 
-    Hint Rewrite map_terms_map : rho.
-
-    Lemma map_brs_map t Γ l H : @map_brs t (fun Γ x Hx => rho Γ x) Γ l H = map (fun x => (x.1, rho Γ x.2)) l. 
-    Proof. 
-      unfold map_brs. now rewrite map_In_spec.
-    Qed. 
-    Hint Rewrite map_brs_map : rho.
-
-    Definition map_fix (rho : context -> term -> term) Γ mfixctx (mfix : mfixpoint term) :=
-      (map (map_def (rho Γ) (rho (Γ ,,, mfixctx))) mfix).
-
-    Lemma map_fix_rho_map t Γ mfix ctx H : 
-      @map_fix_rho t (fun Γ x Hx => rho Γ x) Γ ctx mfix H = 
-      map_fix rho Γ ctx mfix.
-    Proof. 
-      unfold map_fix_rho. now rewrite map_In_spec.
-    Qed. 
-
-    Lemma fold_fix_context_wf_fold mfix Γ ctx :
-      fold_fix_context_wf mfix (fun Γ x _ => rho Γ x) Γ ctx = 
-      fold_fix_context rho Γ ctx mfix.
-    Proof.
-      induction mfix in ctx |- *; simpl; auto. 
-    Qed.
-
-    Hint Rewrite map_fix_rho_map fold_fix_context_wf_fold : rho.
-
-    Lemma mkApps_tApp f a l : mkApps (tApp f a) l = mkApps f (a :: l).
-    Proof. reflexivity. Qed.
-
-    Lemma tApp_mkApps f a : tApp f a = mkApps f [a].
-    Proof. reflexivity. Qed.
-
-    Lemma isFixLambda_app_mkApps t l : isFixLambda_app t -> isFixLambda_app (mkApps t l).
-    Proof. 
-      induction l using rev_ind; simpl; auto.
-      rewrite -mkApps_nested. 
-      intros isf. specialize (IHl isf).
-      simpl. rewrite IHl. destruct (mkApps t l); auto.
-    Qed.
-    Definition isFixLambda (t : term) : bool :=
-    match t with
-    | tFix _ _ => true
-    | tLambda _ _ _ => true
-    | _ => false
-    end.
-
-    Inductive fix_lambda_view : term -> Type :=
-    | fix_lambda_lambda na b t : fix_lambda_view (tLambda na b t)
-    | fix_lambda_fix mfix i : fix_lambda_view (tFix mfix i)
-    | fix_lambda_other t : ~~ isFixLambda t -> fix_lambda_view t.
-
-    Lemma view_fix_lambda (t : term) : fix_lambda_view t.
-    Proof.
-      destruct t; repeat constructor.
-    Qed.
-    
-    Lemma isFixLambda_app_mkApps' t l x : isFixLambda t -> isFixLambda_app (tApp (mkApps t l) x).
-    Proof. 
-      induction l using rev_ind; simpl; auto.
-      destruct t; auto.
-      intros isl. specialize (IHl isl).
-      simpl in IHl.
-      now rewrite -mkApps_nested /=. 
-    Qed.
-
-    Ltac solve_discr := (try (progress (prepare_discr; finish_discr; cbn [mkApps] in * )));
-       try discriminate.
-  
-    Ltac discr_mkApps H := 
-      let Hf := fresh in let Hargs := fresh in
-      rewrite ?tApp_mkApps ?mkApps_nested in H;
-        (eapply mkApps_nApp_inj in H as [Hf Hargs] ||
-         eapply (mkApps_nApp_inj _ _ []) in H as [Hf Hargs] ||
-         eapply (mkApps_nApp_inj _ _ _ []) in H as [Hf Hargs]);
-         [noconf Hf|reflexivity].
-
-    Set Equations With UIP. (* This allows to use decidable equality on terms. *)
-
-    (* Most of this is discrimination, we should have a more robust tactic to  
-      solve this. *)
-    Lemma rho_app_lambda Γ na ty b a l :
-      rho Γ (mkApps (tApp (tLambda na ty b) a) l) =  
-      mkApps ((rho (vass na (rho Γ ty) :: Γ) b) {0 := rho Γ a}) (map (rho Γ) l).
-    Proof.
-      induction l using rev_ind; autorewrite with rho.
-      - set (view := view_lambda_fix_app _ _). clearbody view.
-        depelim view. injection H. intros. discr_mkApps H1.
-        injection H. intros. discr_mkApps H1. subst.
-        now simpl in H; noconf H.
-        simpl in i; discriminate.
-      - simpl. rewrite -mkApps_nested. autorewrite with rho.
-        set (view := view_lambda_fix_app _ _). clearbody view.
-        depelim view. injection H. intros. discr_mkApps H1.
-        injection H. intros. discr_mkApps H1. subst. clear H.
-        remember (mkApps (tApp (tLambda na ty b) a) l).
-        depelim view0. discr_mkApps Heqt.
-        discr_mkApps Heqt. subst. simpl. now autorewrite with rho.
-        subst t. elimtype False. rewrite !tApp_mkApps mkApps_nested in i.
-        rewrite isFixLambda_app_mkApps in i => //.
-        elimtype False; rewrite !tApp_mkApps mkApps_nested in i.
-        rewrite isFixLambda_app_mkApps in i => //.
-    Qed.
-    
-    Lemma map_fix_subst f g mfix :
-      (forall n, tFix (map (map_def f g) mfix) n = f (tFix mfix n)) ->
-      fix_subst (map (map_def f g) mfix) =
-      map f (fix_subst mfix).
-    Proof.
-      unfold fix_subst. intros.
-      rewrite map_length. generalize (#|mfix|) at 1 2. induction n. simpl. reflexivity.
-      simpl. rewrite - IHn. f_equal. apply H.
-    Qed.
-
-    Lemma rho_app_fix Γ mfix idx args :
-      let rhoargs := map (rho Γ) args in
-      rho Γ (mkApps (tFix mfix idx) args) = 
-        match nth_error mfix idx with
-        | Some d => 
-          if is_constructor (rarg d) args then 
-            let fn := (subst0 (map (rho Γ) (fix_subst mfix))) (rho (Γ ,,, fold_fix_context rho Γ [] mfix) (dbody d)) in
-            mkApps fn rhoargs
-          else mkApps (rho Γ (tFix mfix idx)) rhoargs
-        | None => mkApps (rho Γ (tFix mfix idx)) rhoargs
-        end.
-    Proof.
-      induction args using rev_ind; autorewrite with rho.
-      - intros rhoargs.
-        destruct nth_error as [d|] eqn:eqfix => //.
-        rewrite /is_constructor nth_error_nil //.
-      - simpl. rewrite map_app /=.
-        destruct nth_error as [d|] eqn:eqfix => //.
-        destruct (is_constructor (rarg d) (args ++ [x])) eqn:isc.
-        rewrite -mkApps_nested /=.
+  Proof.
+    induction args using rev_ind; autorewrite with rho.
+    - intros rhoargs.
+      destruct nth_error as [d|] eqn:eqfix => //.
+      rewrite /is_constructor nth_error_nil //.
+    - simpl. rewrite map_app /=.
+      destruct nth_error as [d|] eqn:eqfix => //.
+      destruct (is_constructor (rarg d) (args ++ [x])) eqn:isc.
+      rewrite -mkApps_nested /=.
+      autorewrite with rho.
+      set (view := view_lambda_fix_app _ _). clearbody view.
+      depelim view.
+      * injection H; intros Ha Hargs. subst. discr_mkApps Hargs.
+        subst l. noconf H. autorewrite with rho.
+        simpl. autorewrite with rho.
+        unfold unfold_fix.
+        rewrite /map_fix. rewrite nth_error_map.
+        unfold unfold_fix in eqfix.
+        rewrite eqfix /= isc map_app.
+        f_equal => //.
+        rewrite map_fix_subst => //. 
+        intros n.
+        autorewrite with rho. simpl. f_equal.
+        now autorewrite with rho.
+      * injection H. intros _ H'; discr_mkApps H'.
+      * elimtype False; rewrite tApp_mkApps in i.
+        rewrite isFixLambda_app_mkApps' in i => //. 
+      * rewrite -mkApps_nested.
         autorewrite with rho.
-        set (view := view_lambda_fix_app _ _). clearbody view.
-        depelim view.
-        * injection H; intros Ha Hargs. subst. discr_mkApps Hargs.
-          subst l. noconf H. autorewrite with rho.
-          simpl. autorewrite with rho.
+        set (view := view_lambda_fix_app _ _).
+        clearbody view.
+        remember (mkApps (tFix mfix idx) args) as t.
+        destruct view; simpl; try discr_mkApps Heqt.
+        ** subst l. autorewrite with rho.
           unfold unfold_fix.
-          rewrite /map_fix. rewrite nth_error_map.
-          unfold unfold_fix in eqfix.
-          rewrite eqfix /= isc map_app.
-          f_equal => //.
-          rewrite map_fix_subst => //. 
-          intros n.
-          autorewrite with rho. simpl. f_equal.
-          now autorewrite with rho.
-        * injection H. intros _ H'; discr_mkApps H'.
-        * elimtype False; rewrite tApp_mkApps in i.
-          rewrite isFixLambda_app_mkApps' in i => //. 
-        * rewrite -mkApps_nested.
-          autorewrite with rho.
-          set (view := view_lambda_fix_app _ _).
-          clearbody view.
-          remember (mkApps (tFix mfix idx) args) as t.
-          destruct view; simpl; try discr_mkApps Heqt.
-          ** subst l. autorewrite with rho.
-            unfold unfold_fix.
-            rewrite /map_fix nth_error_map eqfix /= isc map_app //.
-          ** subst t. rewrite isFixLambda_app_mkApps' in i => //.
-        * rewrite -mkApps_nested; autorewrite with rho.
-          set (view := view_lambda_fix_app _ _).
-          clearbody view.
-          remember (mkApps (tFix mfix idx) args) as t.
-          destruct view; simpl; try discr_mkApps Heqt.
-          subst l.
-          rewrite /unfold_fix. autorewrite with rho.
-          rewrite /map_fix nth_error_map eqfix /= map_app //.
-          subst t.
-          rewrite isFixLambda_app_mkApps' in i => //.
-      Qed.
+          rewrite /map_fix nth_error_map eqfix /= isc map_app //.
+        ** subst t. rewrite isFixLambda_app_mkApps' in i => //.
+      * rewrite -mkApps_nested; autorewrite with rho.
+        set (view := view_lambda_fix_app _ _).
+        clearbody view.
+        remember (mkApps (tFix mfix idx) args) as t.
+        destruct view; simpl; try discr_mkApps Heqt.
+        subst l.
+        rewrite /unfold_fix. autorewrite with rho.
+        rewrite /map_fix nth_error_map eqfix /= map_app //.
+        subst t.
+        rewrite isFixLambda_app_mkApps' in i => //.
+  Qed.
+
+  Lemma rho_app_case Γ ind pars p x brs :
+    rho Γ (tCase (ind, pars) p x brs) =
+    let (f, args) := decompose_app x in
+    match f with
+    | tConstruct ind' c u => 
+      if eq_inductive ind ind' then
+        let p' := rho Γ p in 
+        let args' := map (rho Γ) args in 
+        let brs' := map (on_snd (rho Γ)) brs in 
+        iota_red pars c args' brs'
+      else tCase (ind, pars) (rho Γ p) (rho Γ x) (map (on_snd (rho Γ)) brs)
+    | tCoFix mfix idx =>
+      match nth_error mfix idx with
+      | Some d => 
+        let fn := (subst0 (map (rho Γ) (cofix_subst mfix))) (rho (Γ ,,, fold_fix_context rho Γ [] mfix) (dbody d)) in
+        tCase (ind, pars) (rho Γ p) (mkApps fn (map (rho Γ) args)) (map (on_snd (rho Γ)) brs)
+      | None => tCase (ind, pars) (rho Γ p) (rho Γ x) (map (on_snd (rho Γ)) brs)
+      end
+    | _ => tCase (ind, pars) (rho Γ p) (rho Γ x) (map (on_snd (rho Γ)) brs)
+    end.
+  Proof.
+    autorewrite with rho.
+    set (app := inspect _).
+    destruct app as [[f l] eqapp].
+    rewrite -{2}eqapp. autorewrite with rho.
+    destruct view_construct_cofix; autorewrite with rho.
+    destruct eq_inductive eqn:eqi; simp rho => //.
+    destruct unfold_cofix as [[rarg fn]|]; simp rho => //.
+    simpl. autorewrite with rho. rewrite /map_fix nth_error_map.
+    destruct nth_error => /=. f_equal.
+    f_equal. rewrite (map_cofix_subst rho (fun x y => rho (x ,,, y))) //.
+    intros. autorewrite with rho. simpl. now autorewrite with rho.
+    reflexivity.
+    simpl.
+    autorewrite with rho.
+    rewrite /map_fix nth_error_map.
+    destruct nth_error => /= //.
+    rewrite (map_cofix_subst rho (fun x y => rho (x ,,, y))) //.
+    intros; simp rho; simpl; now simp rho.
+    simpl. eapply symmetry, decompose_app_inv in eqapp.
+    subst x. destruct t; simpl in d => //.
+  Qed.
+
+  Lemma rho_app_proj Γ ind pars arg x :
+    rho Γ (tProj (ind, pars, arg) x) =
+    let (f, args) := decompose_app x in
+    match f with
+    | tConstruct ind' c u => 
+      if eq_inductive ind ind' then
+        match nth_error args (pars + arg) with
+        | Some arg1 => rho Γ arg1
+        | None => tProj (ind, pars, arg) (rho Γ x)
+        end
+      else tProj (ind, pars, arg) (rho Γ x)
+    | tCoFix mfix idx =>
+      match nth_error mfix idx with
+      | Some d => 
+        let fn := (subst0 (map (rho Γ) (cofix_subst mfix))) (rho (Γ ,,, fold_fix_context rho Γ [] mfix) (dbody d)) in
+        tProj (ind, pars, arg) (mkApps fn (map (rho Γ) args))
+      | None => tProj (ind, pars, arg) (rho Γ x)
+      end
+    | _ => tProj (ind, pars, arg) (rho Γ x)
+    end.
+  Proof.
+    autorewrite with rho.
+    set (app := inspect _).
+    destruct app as [[f l] eqapp].
+    rewrite -{2}eqapp. autorewrite with rho.
+    destruct view_construct_cofix; autorewrite with rho.
+    destruct eq_inductive eqn:eqi; simp rho => //.
+    set (arg' := inspect _). clearbody arg'.
+    destruct arg' as [[arg'|] eqarg'];
+    autorewrite with rho. rewrite eqi.
+    simp rho in eqarg'. rewrite nth_error_map in eqarg'.
+    destruct nth_error => //. now simpl in eqarg'.
+    simp rho in eqarg'; rewrite nth_error_map in eqarg'.
+    destruct nth_error => //.
+    destruct inspect as [[arg'|] eqarg'] => //; simp rho.
+    now rewrite eqi.
+    simpl. autorewrite with rho.
+    rewrite /map_fix nth_error_map.
+    destruct nth_error eqn:nth => /= //.
+    f_equal. f_equal. f_equal.
+    rewrite (map_cofix_subst rho (fun x y => rho (x ,,, y))) //.
+    intros. autorewrite with rho. simpl. now autorewrite with rho.
+    simpl. eapply symmetry, decompose_app_inv in eqapp.
+    subst x. destruct t; simpl in d => //.
+  Qed.
+
+  
